The *"regular" chain rule*:

If $\large{y = f(g(x))}$, then:
$\large{y = f(u)}$, and $\large{u = g(x)}$

![[11. Multivariable Chain Rule 2024-02-15 08.12.16.excalidraw]]

and $\large{\dfrac{dy}{dx} = \dfrac{dy}{du} \cdot \dfrac{du}{dx}}$

Now, suppose $\large{z = f(x,y)}$ and $\large{y = g(t)}$, $\large{y = h(t)}$

![[11. Multivariable Chain Rule 2024-02-15 08.15.49.excalidraw|800]]

What if $\large{w = f(x,y,z)}$, $\large{x = g(s, t)}$, $\large{y = h(s,t)}$, $\large{z = k(s,t)}$?

![[11. Multivariable Chain Rule 2024-02-15 08.19.57.excalidraw]]

$\large{\dfrac{\partial w}{\partial s} = \dfrac{\partial w}{\partial x} \cdot \dfrac{\partial x}{\partial s} + \dfrac{\partial w}{\partial y} \cdot \dfrac{\partial y}{\partial s} + \dfrac{\partial w}{\partial z} \cdot \dfrac{\partial z}{\partial s}}$

$\large{\dfrac{\partial w}{\partial t} = \dfrac{\partial w}{\partial x} \cdot \dfrac{\partial x}{\partial t} + \dfrac{\partial w}{\partial y} \cdot \dfrac{\partial y}{\partial t} + \dfrac{\partial w}{\partial z} \cdot \dfrac{\partial z}{\partial t}}$

___

>[!question] 15.9
>Find $\large{\dfrac{dz}{dt}}$ if $\large{z = x\sin(y)}$, $\large{x = t^2}$, $\large{y = 4t^3}$.

>[!check]- Solution
>$\large{\dfrac{dz}{dt} = \dfrac{dx}{dt} \cdot \dfrac{\partial z}{\partial x} + \dfrac{dy}{dt} \cdot \dfrac{\partial z}{\partial y} = \sin(y)\cdot(2t) + x\cos(y)\cdot12t^2}$

>[!question] 13
>Find $\large{\dfrac{dz}{dt}}$ if $\large{z = (x+2y)^10}$, $\large{x = sin^2(t)}$, $\large{y = (3t+4)^5}$

>[!check]- Solution
>$\large{\begin{align} \dfrac{dz}{dt} &= \dfrac{dx}{dt} \cdot \dfrac{\partial z}{\partial x} + \dfrac{dy}{dt} \cdot \dfrac{\partial z}{\partial y} \\ \\  &= 10(x+2y)^9\cdot1\cdot2\sin(t)\cdot\cos(t) + 10(c+2y)^9\cdot2\cdot5(3t+4)^4\cdot3 \\ \\ &= 20(x+2y)^9(\sin(t)\cos(t)+15(3t+4)^4) \end{align}}$

>[!question] 25
>Find $\large{\dfrac{\partial w}{\partial s}}$ and $\large{\dfrac{\partial w}{\partial t}}$ if 
>
>$\large{w = \dfrac{x - z}{y+z}, x = s + t, y + st, z = s - t}$

>[!check]- Solution
>$\large{\dfrac{\partial w}{\partial s} = \dfrac{\partial w}{\partial x} \cdot \dfrac{\partial x}{\partial s} + \dfrac{\partial w}{\partial y} \cdot \dfrac{\partial y}{\partial s} + \dfrac{\partial w}{\partial z} \cdot \dfrac{\partial z}{\partial s}}$
>
>$\large{\dfrac{\partial w}{\partial x} = \dfrac{1}{y+z}}$
>
>$\large{\dfrac{\partial w}{\partial y} = -(x-z)(y+z)^{-2}}$
>
>$\large{\dfrac{\partial w}{\partial z} = \dfrac{d}{dz}(\dfrac{x-z}{y+z}) = \dfrac{-y-z - x + z)}{y+z}^2 = \dfrac{-y-x}{(y+z)^2}}$
> 
> $\large{\dfrac{\partial x}{\partial s} = 1, \dfrac{\partial y}{\partial s} = t, \dfrac{\partial z}{\partial s} = 1}$
> 
> So $\large{\dfrac{\partial w}{\partial s} = \dfrac{1}{y+z} + \dfrac{z-x}{(y+z)^2} \cdot t + \dfrac{-y-x}{(y+z)^2} = \dfrac{(z-x)(1+t)}{(y+z)^2}}$

___

## Theorem 15.9 Implicit Differentiation
Let $\large{F}$ be differentiable on its domain and suppose $\large{F(x,y) = k}$ defines $\large{y}$ as a differentiable function of $\large{x}$. Provided $\large{F_y \neq 0}$
$$\large{\dfrac{dy}{dx} = -\dfrac{F_x}{F_y}}$$

**Explanation:**
Let us suppose
$\large{F(x,y) = k}$

$\large{\dfrac{d}{dx}(F(x,y)) = \dfrac{d}{dx}(k)}$

$\large{\dfrac{dF}{dx} = \dfrac{\partial F}{\partial x} + \dfrac{\partial F}{\partial y} \cdot \dfrac{dy}{dx}}$

So $\large{\dfrac{dy}{dx} = -\dfrac{\frac{\partial F}{\partial x}}{\frac{\partial F}{\partial y}}}$ 

___

For $\large{F(x,y,z) = k}$, $\large{\dfrac{\partial z}{\partial x} = - \dfrac{\partial F_x}{\partial F_z}, \dfrac{\partial z}{\partial y} = -\dfrac{\partial F_y}{\partial F_z}}$

>[!question] 57
> Use the above results to find
> $\large{\dfrac{\partial z}{\partial x}}$ and $\large{\dfrac{\partial z}{\partial y}}$ fo $\large{xy+xz+yz = 3}$

>[!check]- Solution
>$\large{\dfrac{\partial z}{\partial x} = -\dfrac{F_x}{F_z} = -\dfrac{y+z}{x+z}}$, $\large{\dfrac{\partial z}{\partial y} = -\dfrac{F_y}{F_z} = -\dfrac{(x+z)}{x+y}}$