**Recall:**
- Any equation of the form $\large{F(x,y,z) = k}$ has a surface

The **Tangent Plane** to $\large{F(x,y,z) = k}$
![[13. Tangent Planes and Linear Approximation 2024-02-22 08.18.03.excalidraw|800]]

Remember, **GRADIENT IS ALWAYS ORTHOGONAL TO TANGENT PLANE**.

## Definition: Equation of The Tangent Plane for $\large{F(x,y,z) = 0}$
Let $\large{F}$ be differentiable at the point $\large{P_0(a,b,c)}$ with $\large{\nabla F(a,b,c) \neq 0}$. The plane tangent to the surface $\large{F(x,y,z) = 0}$ at $\large{P_0}$, called the **tangent plane**, is the plane passing through $\large{P}$ orthogonal to the gradient.

What about the tangent plane to the graph of $\large{z = f(x,y)}$ at the point $\large{(a,b, f(a,b))}$?

so a normal vector (at point on surface) is:
$\large{\nabla F = \langle F_x, F_y, F_z \rangle = \langle - f_x, -f_y, 1 \rangle}$,
so tangent plane equation at $\large{P(a,b,f(a,b))}$ is
$$\large{-f_x(a,b)(x-a) - f_y(a,b)(y-b) + (z-c) = 0}$$
$$\large{\implies z = f(a,b) + f_x(a,b)(x-a) + f_y(a,b)(y-b)}$$

Note $\large{z-c = f(a,b)}$

___

**Tangent Plane** for $\large{z = f(x,y)}$
Let $\large{f}$ be differentiable at the point $\large{(a,b)}$. An equation of the plane tangent to the surface $\large{z = f(x,y)}$ at the point $\large{(a,b,f(a,b))}$ is
$$\large{z = f_x(a,b)(x-a) + f_y(a,b)(y-b) + f(a,b)}$$

___

>[!question] 15.6 (22)
>Find an equation for the plane tangent to $\large{yze^{xz} - 8 = 0}$ at the point $\large{(0,2,4)}$.

>[!check]- Solution
>$\large{\begin{align} \nabla F &= \langle F_x, F_y, F_z \rangle = \langle yz\cdot e^{xz} \cdot z, ze^{xz}, yz\cdot e^{xz}\cdot x + e^{xz} \cdot y \\ &= \langle yz^2e^{xz}, ze^{xz}, ye^{xz}(xz+1) \rangle\end{align}}$
> 
> $\large{\nabla F(0,2,4) = \langle 32, 4, 2 \rangle}$, so tangent plane is
> $\large{32(x-0) + 4(y-2) + 2(z-4) = 0 = 16x + 2(y-2) + (z-2)}$

>[!question] 29
>Find an equation for the plane tangent to $\large{z = \tan^{-1}(xy)}$ at the point $\large{(1,1, \dfrac{\pi}{4})}$.

>[!check]- Solution
>Tangent Plane: $\large{z = f(a,b) + f_x(a,b)(x-a) + f_y(a,b)(y-b)}$
>$\large{f(a,b) = f(1,1) = \tan^{-1}(1) = \dfrac{\pi}{4}}$ - Checking to see if the point is on the plane. It is.
>$\large{f_x = \dfrac{1}{1+(xy)^2}\cdot y, f_x(1,1) = \dfrac{1}{2}}$
>$\large{f_y = \dfrac{1}{1 + (xy)^2} \cdot x, f_y(1,1) = \dfrac{1}{2}}$
> 
> So tangent plane is:
> $\large{z = \dfrac{\pi}{4} + \dfrac{1}{2}(x-1) + \dfrac{1}{2}(y-1)}$

**Recall:**
"Linear Approximation" from Calculus I:

![[13. Tangent Planes and Linear Approximation 2024-02-22 08.40.01.excalidraw|800]]

![[13. Tangent Planes and Linear Approximation 2024-02-22 08.43.28.excalidraw|800]]

## Definition: The differential $\large{dz}$
Let $\large{f}$ be differentiable at the point $\large{(x,y)}$. The change in $\large{z = f(x,y)}$ as the independent variables change from $\large{(x,y)}$ to $\large{(x+dx, y+dy)}$ is denoted $\large{\Delta z}$ and is approximated by the differential
$$\large{\Delta z \approx dz = f_x(x,y)dx + f_y(x,y)dy}$$

>[!question] 15.6 (35)
>**a)** Find the linear approximation to $\large{f(x,y) = -x^2+2y^2}$ at $\large{(3,-1)}$
>**b)** Use part (a) to estimate $\large{f(3.1, -1.04)}$

>[!check]- Solution
>**a)** $\large{L(x,y) = f(a,b) + f_x(a,b)(x-a) + f_y(a,b)(y-b)}$
>$\large{f(a,b) = f(3,-1) = -9 + 2 = -7}$
>$\large{f_x = -2x, f_x(3,-1) = -6}$
>$\large{f_y = 4y, f_y (3,-1) = -4}$
>so $\large{L(x,y) = -7-6(x-3) - 4(y+1)}$
>
>**b)** $\large{f(3.1,-1.04) \approx L(3.1,-1.04) = -7.44}$

>[!question] (55)
>Find the points at which the surface $\large{x^2+y^2 - z^2 - 2x + 2y + 3 = 0}$ has horizontal tangent planes.

>[!check]- Solution
>The given surface is a level surface, for $\large{F(x,y,z) = x^2+y^2 - z^2 - 2x + 2y + 3}$
>We'll search for points where the gradient vector is vertical, meaning $\large{\nabla F(P) = \langle 0, 0, \_ \rangle}$
> 
> $\large{\implies F_x(a,b,c) = 0,\;F_y(a,b,c) = 0,\;F(a,b,c) = 0}$
> $\large{\implies 2x-2 = 0, 2y + 2 = 0, x^2+y^2 - z^2 - 2x + 2y + 3 = 0}$
> $\large{\implies x = 1, y = -1}$
> 
> $\large{1 + 1 - z^2 - 2 - 2 + 3 = 0 \implies z^2 = 1 \implies z = \pm 1}$
> So the points are: $\large{(1,-1,1), (1,-1,-1)}$

>[!question] 15.6
>a) The volume of a right circular cone with radius $\large{r}$ and a height $\large{h}$ is $\large{V = \dfrac{1}{3}\pi r^2 h}$. Approximate the change in the volume of such a cone when radius changes from $\large{r = 6.5}$ to $\large{r = 6.6}$ and height changes from $\large{h = 4.20}$ to $\large{h = 4.15}$

>[!check]- Solution
>When they're small, $\large{\Delta V = dV}$
>Here
>$\large{\Delta V = \dfrac{1}{3} \pi (6.6)^2 (4.15) - \dfrac{1}{3}\pi(6.5)^2(4.20)}$
>$\large{dV = V_r\cdot dr + V_h \cdot dh}$ where $\large{V(r,h) = \dfrac{1}{3}\pi r^2 h}$
>$\large{dV = (\dfrac{2}{3}\pi r h) \cdot dr + \dfrac{1}{3}\pi r^2 \cdot dh = \dfrac{2}{3}\pi \cdot 6.5 \cdot 4.2 \cdot 0.1 + \dfrac{1}{3}\pi \cdot 6.5^2 \cdot (-0.05)}$

