For $\large{f(x,y)}$, the partial derivative of $\large{f}$ with respect to $\large{x}$, denoted $\large{\dfrac{\partial f}{\partial x}}$, represents the instantaneous rate of change of $\large{f(x,y)}$ with respect to x *while holding y fixed*. That is

$$\large{\dfrac{\partial f}{\partial x} = \lim_{h\to0}\dfrac{f(x+h,y)-f(x,y)}{h}}$$

$\large{\dfrac{\partial f}{\partial x}}$ is found by applying known derivative rules to the $\large{f(x,y)}$ expression while treating the character $\large{y}$ as if it represents a constant

>[!question] Example
>For $\large{f(x,y) = x^2+2xy+y^3}$

>[!check]- Solution
>$\large{\dfrac{\partial f}{\partial x} = \dfrac{d}{dx}(x^2+2y+y^3) = 2x+2\cdot1\cdot y+0 = 2x+2y}$

Similarly,
$$\large{\dfrac{\partial f}{\partial y} = \lim_{h\to0}\dfrac{f(x,y+h)-f(x,y)}{h}}$$

and $\large{\dfrac{\partial f}{\partial y}}$ is found by using known derivative rules while treating $\large{y}$ as the variable and $\large{x}$ as the constant.

>[!question] Example
>For $\large{f(x,y) = x^2+2xy+y^3}$

>[!check]- Solution
>$\large{\dfrac{\partial f}{\partial y} = \dfrac{d}{dy}(x^2+2xy+y^3) = 0 +2x\cdot 1 + 3y^2 = 2x+3y^2}$

Graphically:

![[9. Partial Derivatives 2024-02-08 08.23.23.excalidraw]]

Notation: partial derivatives at arbitrary variable (x,y):

$$\large{\dfrac{\partial f}{\partial x}(x,y)=\dfrac{\partial f}{\partial x}=f_x(x,y) = f_x}$$

$$\large{\dfrac{\partial f}{\partial y}(x,y)=\dfrac{\partial f}{\partial y}=f_y(x,y) = f_y}$$

At a specific point:

$$\large{\dfrac{\partial f}{\partial x}(2,1)=\dfrac{\partial f}{\partial y}\rvert_{(2,1)}=f_x(2,1)}$$

$\large{\dfrac{df}{dx}}$ "ordinary" derivative, indicates that $\large{f}$ has only one input variable, x.

$\large{\dfrac{\partial f}{\partial x}}$ "partial" derivative, indicates that $\large{f}$ has inputs other than the variable, x.

>[!question] 15.3 (16)
>Find the partial derivatives for $\large{f(x,y) = 4x^3y^2+3x^2y^3 + 10}$

>[!check]- Solution
>$\large{\dfrac{\partial f}{\partial x} = f_x = \dfrac{d}{dx}(4x^3y^2 + 3x^2y^3 + 10) = 12x^2y^2 + 6xy^3}$
>
>$\large{\dfrac{\partial f}{\partial y} = f_y = \dfrac{d}{dy}(4x^3y^2 + 3x^2y^3 + 10) = 8x^3y+9xy^2}$ 

**NOTE:** Constant with the variable derived it comes with, if by itself it becomes 0.
$\large{\dfrac{\partial}{\partial y}(4x^3y^2) = 4x^3 \cdot 2y}$
$\large{\dfrac{\partial}{\partial y}(4x^3+y^2 = 0 + 2y = 2y)}$

>[!question] 17
>Find the partial derivatives for $\large{f(x,y) = e^{x^2y}}$

>[!check]- Solution
>$\large{f_x = \dfrac{\partial}{\partial x}(e^{x^2y}) = e^{x^2y} \cdot \dfrac{\partial}{\partial x}(x^2y) = e^{x^2y}(2xy) = 2xye^{x^2y}}$
>
>$\large{f_y = \dfrac{\partial}{\partial y} = e^{x^2y}\dfrac{\partial}{\partial y}(x^2y) = e^{x^2y}\cdot x^2 = x^2e^{x^2y}}$

>[!question] (29)
>Find the partial derivatives for $\large{g(x,z) = x\ln(x^2+z^2)}$

>[!check]- Solution
>$\large{\begin{align} g_x &= \dfrac{\partial}{\partial x}(x\cdot\ln(x^2+z^2)) = x\cdot\dfrac{\partial}{\partial x}(\ln(x^2+z^2)) + \ln(x^2+z^2) \cdot \dfrac{\partial}{\partial x}(x) \\ \\ &= x\cdot \dfrac{1}{x^2+z^2}\cdot(2x + 0) + \ln(x^2+z^2)\cdot 1 = \dfrac{2x^2}{x^2+z^2} + \ln(x^2+z^2) \end{align}}$
> 
> $\large{g_z = \dfrac{\partial}{\partial z}(x\cdot\ln(x^2+z^2)) = x\cdot\dfrac{\partial}{\partial z}(\ln(x^2+z^2)) = x\cdot\dfrac{1}{x^2+z^2}\cdot(0 + 2z) = \dfrac{2xz}{x^2+z^2}}$

>[!question] (40)
Find all four *second-order* partial derivatives for $\large{f(x,y) = 2x^3y^2 + x^2y}$

>[!check]- Solution
> $\large{(f_x)_x,\;(f_x)_y,\;(f_y)_x,\;(f_y)_y}$ are the four *second-order* partial derivatives
> 
> $\large{f_x = 10x^4y^2 + 2xy}$
> $\large{f_y = 2x^5\cdot2y + x^2 \cdot 1 = 4x^5y + x^2}$
> 
> 1. $\large{f_{xx}}$
> $\large{\begin{align} (f_x)_x &= f_{xx} = \dfrac{d}{dx}\left(\dfrac{\partial f}{\partial x}\right) = \dfrac{\partial^2 f}{\partial x^2} = \dfrac{\partial}{\partial x} (f_x) = \dfrac{\partial}{\partial x}(10x^2y^2 + 2xy) \\ &= 40x^2y^2 + 2y \end{align}}$
> 
> 2. $\large{f_{xy}}$
> $\large{\begin{align} (f_x)_y &= f_{xy} = \dfrac{d}{dy}\left(\dfrac{\partial f}{\partial x }\right) = \dfrac{\partial^2 f}{\partial y \partial x} = \dfrac{\partial}{\partial y} (f_x) = \dfrac{\partial}{\partial x}(10x^2y^2 + 2xy) \\ &= 10x^4\cdot2y + 2y = 20x^4y + 2y \end{align}}$
> 
> 3. $\large{f_{yy}}$
>$\large{(f_y)_y = f_{yy} = \dfrac{d}{dy} = \dfrac{\partial}{\partial y} (f_y) = \dfrac{\partial}{\partial y}(4x^5y+x^2) = 4x^5 + 0 = 4x^5}$
> 
> 4. $\large{f_{yx}}$
>$\large{(f_y)_x = f_{yx} = \dfrac{\partial }{\partial y}(4x^5y + x^2) = 20x^4y + 2x}$

**NOTE:** For our purposes, as we deal with mainly polynomials, trigonometric functions, exponential functions, etc,
$$\large{f_{xy} = f_{yx}}$$

## Definition: Differentiability

The function $\large{z = f(x,y)}$ os **differentiable** at $\large{(a,b)}$ provided $\large{f_x(a,b)}$ and $\large{f_y(a,b)}$ exist and the change $\large{\Delta z = f(a + \Delta x, b + \Delta y) - f(a,b)}$ equals
$$\large{\Delta z = }$$

trace on the graph of $\large{f}$ is tangent to the plane.

## Theorem 15.5 Conditions for Differentiability
Suppose the function $\large{f}$ has partial derivatives $\large{f_x}$ and $\large{f_y}$ defined on an open set containing $\large{(a,b)}$, with $\large{f_x}$ and $\large{f_y}$ continuous at $\large{(a,b)}$. Then $\large{f}$ is differentiable at $\large{(a,b)}$

## Theorem 15.6 Differentiable Implies Continuous
If a function $\large{f}$ is differentiable at $\large{(a,b)}$, then it is continuous at $\large{(a,b)}$.